io/Compiler.Languages.fst
@@ -2,12 +2,13 @@ module Compiler.Languages
 
 open FStar.Tactics
 open FStar.Tactics.Typeclasses
+open FStar.Ghost
 
 open CommonUtils
 open TC.Monitorable.Hist
 
 (** ** IIO **)
-include IIO
+include IIO2
 
 (** ** ILang **)
 (** ILang is a language that acts as an intermediate language between the rich IIO effect that has
@@ -24,8 +25,8 @@ include IIO
 **)
 
 
-effect IIOpi (a:Type) (pi : monitorable_prop) = 
-  IIO.IIOwp a (pi_as_hist #a pi)
+effect IIOpi (a:Type) (fl:FStar.Ghost.erased tflag) (pi : monitorable_prop) = 
+  IIOwp a fl (pi_as_hist #a pi)
 
 class ilang (t:Type u#a) (pi:monitorable_prop) = { [@@@no_method] mldummy : unit }
 
@@ -43,13 +44,13 @@ instance ilang_either (pi:monitorable_prop) t1 {| d1:ilang t1 pi |} t2 {| d2:ila
 instance ilang_resexn (pi:monitorable_prop) t1 {| d1:ilang t1 pi |} : ilang (resexn t1) pi =
   { mldummy = () }
 
-type ilang_arrow_typ (t1 t2:Type) pi = t1 -> IIOpi t2 pi
+type ilang_arrow_typ (fl:erased tflag) (t1 t2:Type) pi = t1 -> IIOpi t2 fl pi
 
 (** An ilang arrow is a statically verified arrow to respect pi.
     It can expect an argument that respects a different pi1, or it
     can return a function that respects pi2. 
 **)
-instance ilang_arrow (#pi1 #pi2 pi:monitorable_prop) #t1 (d1:ilang t1 pi1) #t2 (d2:ilang t2 pi2) : ilang (ilang_arrow_typ t1 t2 pi) pi =
+instance ilang_arrow (#fl:erased tflag) (#pi1 #pi2 pi:monitorable_prop) #t1 (d1:ilang t1 pi1) #t2 (d2:ilang t2 pi2) : ilang (ilang_arrow_typ fl t1 t2 pi) pi =
   { mldummy = () }
 
 (**instance ilang_fo_uint8 : ilang_fo UInt8.t = { fo_pred = () }
@@ -153,6 +154,18 @@ instance mlang_effectpoly
   mlang (mon:monad -> acts mon -> ct mon.m) =
   { mldummy = () }
 
+let dm_mon (pi:monitorable_prop) : monad = {
+  m = rilang_dm pi;
+  ret = (fun (x:'a) -> IIO.dm_iio_return 'a x);
+  bind = (fun (m:rilang_dm pi 'a) (k:'a -> rilang_dm pi 'b) -> 
+    let wp : Hist.hist 'b = Hist.hist_bind (pi_as_hist #'a pi) (fun _ -> pi_as_hist pi) in 
+    let tr : IIO.dm_iio 'b wp = IIO.dm_iio_bind _ _ _ _ (as_iio_dm m) (fun x -> as_iio_dm (k x)) in
+    lemma_bind_pi_implies_pi #'a #'b pi;
+    let w = IIO.dm_iio_subcomp 'b wp (pi_as_hist pi) tr in
+    as_rilang_dm w)
+}
+
+assume val dm_acts (pi:monitorable_prop) : acts (dm_mon pi)
 
 
 (** *** Manual tests *)
