io/IIO2.fst
@@ -181,6 +181,7 @@ let performance_test (#fl:tflag) : IIOwp unit (fl+IOActions) (fun p h -> forall 
 type rc_typ (t1 t2:Type) = t1 -> trace -> t2 -> trace -> bool
 
 type eff_rc_typ_cont (fl:erased tflag) (t1:Type u#a) (t2:Type u#b) (rc:rc_typ t1 t2) (x:t1) (initial_h:erased trace) =
+  y:t2 -> IIO ((erased trace) * bool) fl (fun h -> (initial_h `suffix_of` h)) (fun h (the_lt, b) lt -> apply_changes initial_h the_lt == h /\ lt == [] /\ (b <==> rc x initial_h y the_lt))
   
 type eff_rc_typ (fl:erased tflag) (t1 t2:Type) (rc:rc_typ t1 t2) =
   x:t1 -> IIO (initial_h:(erased trace) & eff_rc_typ_cont fl t1 t2 rc x initial_h) fl (fun _ -> True) (fun h (| initial_h, _ |) lt -> h == reveal initial_h /\ lt == [])
